coq/theories/ecc.v
@@ -1,0 +1,541 @@
+From mathcomp Require Import ssreflect ssrbool eqtype ssrnat seq.
+From Coq Require Import ssrfun Program Logic.Classical_Prop.
+Require Import AutosubstSsr ARS.
+
+Set Implicit Arguments.
+Unset Strict Implicit.
+Unset Printing Implicit Defensive.
+
+Module ECC.
+
+Declare Scope coc_scope.
+Open Scope coc_scope.
+
+Definition context T := seq (option T).
+Definition cons_Some T (n : T) (Gamma : context T) : context T := 
+  Some n :: Gamma.
+Definition cons_None T (Gamma : context T) : context T := 
+  None :: Gamma.
+
+Notation "m :s Gamma" := (cons_Some m Gamma) (at level 30).
+Notation ":n Gamma" := (cons_None Gamma) (at level 30).
+
+Inductive has {T} `{Ids T} `{Subst T} : 
+  context T -> var -> T -> Prop :=
+| has_O m Gamma :
+  has (m :s Gamma) 0 m.[ren (+1)]
+| has_S Gamma v m n : 
+  has Gamma v m ->
+  has (n :s Gamma) (v.+1) m.[ren (+1)]
+| has_N Gamma v m : 
+  has Gamma v m ->
+  has (:n Gamma) (v.+1) m.[ren (+1)].
+
+Lemma has_x {T} `{Ids T} `{Subst T} (Gamma : context T) x A :
+  has Gamma x A ->
+  forall B,
+    has Gamma x B ->
+    A = B.
+Proof.
+  induction 1; intros.
+  inv H1; eauto.
+  inv H2; eauto.
+  apply IHhas in H7. rewrite H7; eauto.
+  inv H2; eauto.
+  apply IHhas in H5. rewrite H5; eauto.
+Qed.
+  
+Inductive term : Type :=
+| Var (x : var)
+| Sort (n : nat)
+| App  (s t : term)
+| Lam  (s : {bind term})
+| Prod (s : term) (t : {bind term}).
+
+Instance Ids_term : Ids term. derive. Defined.
+Instance Rename_term : Rename term. derive. Defined.
+Instance Subst_term : Subst term. derive. Defined.
+Instance substLemmas_term : SubstLemmas term. derive. Qed.
+
+Inductive value : term -> Prop :=
+| value_sort l   : value (Sort l)
+| value_var x    : value (Var x)
+| value_prod A B : value (Prod A B)
+| value_lam n    : value (Lam n).
+
+Inductive step : term -> term -> Prop :=
+| step_beta s t :
+  step (App (Lam s) t) s.[t/]
+| step_appL s1 s2 t :
+  step s1 s2 ->
+  step (App s1 t) (App s2 t)
+| step_appR s t1 t2 :
+  step t1 t2 ->
+  step (App s t1) (App s t2).
+
+Inductive pstep : term -> term -> Prop :=
+| pstep_var x :
+  pstep (Var x) (Var x)
+| pstep_sort n :
+  pstep (Sort n) (Sort n)
+| pstep_lam s1 s2 :
+  pstep s1 s2 ->
+  pstep (Lam s1) (Lam s2)
+| pstep_beta s1 s2 t1 t2 :
+  pstep s1 s2 ->
+  pstep t1 t2 ->
+  pstep (App (Lam s1) t1) s2.[t2/]
+| pstep_app s1 s2 t1 t2 :
+  pstep s1 s2 ->
+  pstep t1 t2 ->
+  pstep (App s1 t1) (App s2 t2)
+| pstep_prod s1 s2 t1 t2 :
+  pstep s1 s2 ->
+  pstep t1 t2 ->
+  pstep (Prod s1 t1) (Prod s2 t2).
+
+Notation red := (star pstep).
+Notation "s === t" := (conv pstep s t) (at level 50).
+
+Definition psstep (sigma tau : var -> term) :=
+  forall x, pstep (sigma x) (tau x).
+
+Fixpoint rho (s : term) : term :=
+  match s with
+    | App (Lam s) t => (rho s).[rho t/]
+    | App s t => App (rho s) (rho t)
+    | Lam s => Lam (rho s)
+    | Prod A B => Prod (rho A) (rho B)
+    | x => x
+  end.
+
+Lemma pstep_refl s : pstep s s.
+Proof. elim: s; eauto using pstep. Qed.
+Hint Resolve pstep_refl.
+
+Lemma step_pstep s t : step s t -> pstep s t.
+Proof. elim; eauto using pstep. Qed.
+
+Lemma pstep_subst sigma s t :
+  pstep s t -> pstep s.[sigma] t.[sigma].
+Proof.
+  move=> A. elim: A sigma => /=; eauto using pstep.
+  move=> s1 s2 t1 t2 p1 ih1 p2 ih2 sigma. 
+  replace (s2.[t2/].[sigma]) 
+    with (s2.[up sigma].[t2.[sigma]/]) by autosubst.
+  apply pstep_beta; eauto.
+Qed.
+
+Lemma pstep_ren s s' xi :
+  pstep s s' -> pstep s.[ren xi] s'.[ren xi].
+Proof.
+  apply pstep_subst.
+Qed.
+
+Lemma psstep_up sigma tau :
+  psstep sigma tau -> psstep (up sigma) (up tau).
+Proof.
+  move=> A [|n] //=. asimpl. apply: pstep_subst. exact: A.
+Qed.
+
+Lemma pstep_compat sigma tau s t :
+  psstep sigma tau -> pstep s t -> pstep s.[sigma] t.[tau].
+Proof with eauto using pstep, psstep_up.
+  move=> A B. elim: B sigma tau A; asimpl...
+  move=> s1 s2 t1 t2 _ A _ B sigma tau C.
+  replace (s2.[t2/].[tau]) 
+    with (s2.[up tau].[t2.[tau]/]) by autosubst.
+  apply pstep_beta; asimpl...
+Qed.
+
+Lemma pstep_compat_beta s1 s2 t1 t2 :
+  pstep s1 s2 -> pstep t1 t2 -> pstep s1.[t1/] s2.[t2/].
+Proof.
+  move=> A B. by apply: pstep_compat A => -[|].
+Qed.
+
+Lemma rho_triangle : triangle pstep rho.
+Proof with eauto using pstep.
+  move=> s t. elim=> {s t} //=...
+  - move=> s1 s2 t1 t2 _ A _ B. exact: pstep_compat_beta.
+  - move=> s1 s2 t1 t2 A ih1 _ ih2. case: s1 A ih1 => //=...
+    move=> s A ih1. inv A. inv ih1...
+Qed.
+
+Theorem church_rosser :
+  CR pstep.
+Proof with eauto using star.
+  apply: (cr_method (e2 := pstep) (rho := rho))...
+  exact: rho_triangle.
+Qed.
+Hint Resolve church_rosser.
+
+Definition sconv (sigma tau : var -> term) :=
+  forall x, sigma x === tau x.
+
+Lemma conv_app s1 s2 t1 t2 :
+  s1 === s2 -> t1 === t2 -> App s1 t1 === App s2 t2.
+Proof.
+  move=> A B. apply: (conv_trans (App s2 t1)).
+  - apply: (conv_hom (App^~ t1)) A => x y p. by apply: pstep_app.
+  - apply: conv_hom B => x y p. by apply: pstep_app.
+Qed.
+
+Lemma conv_lam s1 s2 : s1 === s2 -> Lam s1 === Lam s2.
+Proof. apply: conv_hom => x y. exact: pstep_lam. Qed.
+
+Lemma conv_prod s1 s2 t1 t2 :
+  s1 === s2 -> t1 === t2 -> Prod s1 t1 === Prod s2 t2.
+Proof.
+  move=> A B. apply: (conv_trans (Prod s2 t1)).
+  - apply: (conv_hom (Prod^~ t1)) A => x y p. by apply: pstep_prod.
+  - apply: conv_hom B => x y p. by apply: pstep_prod.
+Qed.
+
+Lemma conv_subst sigma s t : s === t -> s.[sigma] === t.[sigma].
+Proof. apply: conv_hom. intros. apply: pstep_subst. eauto. Qed.
+
+Definition left_invertible (f : nat -> nat) := 
+  exists g, g ∘ f = id.
+
+Lemma left_invertible_upren xi :
+  left_invertible xi -> left_invertible (upren xi).
+Proof.
+  unfold left_invertible.
+  intros.
+  inv H.
+  exists (upren x).
+  assert (upren x ∘ upren xi = upren xi >>> upren x) by autosubst.
+  rewrite H; asimpl.
+  replace (xi >>> x) with (x ∘ xi) by autosubst.
+  rewrite H0; autosubst.
+Qed.
+
+Lemma sort_ren_inv l v xi :
+  Sort l = v.[ren xi] -> v = Sort l.
+Proof.
+  induction v; asimpl; try discriminate; eauto.
+Qed.
+
+Lemma var_ren_inv x v xi :
+  Var x = v.[ren xi] -> exists n, v = Var n.
+Proof.
+  induction v; asimpl; try discriminate; eauto.
+Qed.
+
+Lemma prod_ren_inv A B v xi :
+  Prod A B = v.[ren xi] -> exists A' B', v = Prod A' B'.
+Proof.
+  induction v; asimpl; try discriminate; eauto.
+Qed.
+
+Lemma lam_ren_inv m v xi :
+  Lam m = v.[ren xi] -> exists n, v = Lam n.
+Proof.
+  induction v; asimpl; try discriminate; eauto.
+Qed.
+
+Lemma value_rename v xi :
+  value v <-> value v.[ren xi].
+Proof.
+  split.
+  induction 1; asimpl; constructor.
+  intros.
+  dependent induction H.
+  apply sort_ren_inv in x; subst.
+  constructor.
+  apply var_ren_inv in x.
+  inv x.
+  constructor.
+  apply prod_ren_inv in x.
+  inv x. inv H.
+  constructor.
+  apply lam_ren_inv in x.
+  inv x.
+  constructor.
+Qed.
+
+Lemma red_sort_inv s A :
+  red (Sort s) A -> A = (Sort s).
+Proof.
+  induction 1; intros; eauto.
+  rewrite IHstar in H0.
+  inv H0; eauto.
+Qed.
+
+Lemma red_prod_inv A B x :
+  red (Prod A B) x -> 
+  exists A' B',
+    red A A' /\
+    red B B' /\
+    x = Prod A' B'.
+Proof.
+  induction 1.
+  - exists A.
+    exists B.
+    repeat constructor.
+  - firstorder.
+    rewrite H3 in H0.
+    inv H0.
+    exists s2.
+    exists t2.
+    repeat constructor; eauto using star.
+Qed.
+
+Ltac red_inv m H :=
+  match m with
+  | Sort   => apply red_sort_inv in H
+  | Prod => apply red_prod_inv in H
+  end.
+
+Ltac solve_conv' :=
+  unfold not; intros;
+  match goal with
+  | [ H : _ === _ |- _ ] =>
+    apply church_rosser in H; inv H
+  end;
+  repeat match goal with
+  | [ H : red (?m _) _ |- _ ] => red_inv m H
+  | [ H : red (?m _ _) _ |- _ ] => red_inv m H
+  | [ H : red (?m _ _ _) _ |- _ ] => red_inv m H
+  end;
+  firstorder; subst;
+  match goal with
+  | [ H : _ = _ |- _ ] => inv H
+  end.
+
+Ltac solve_conv :=
+  match goal with
+  | [ H : ?t1 === ?t2 |- _ ] =>
+    assert (~ t1 === t2) by solve_conv'
+  | [ H : value (App _ _) |- _ ] => inv H
+  end; eauto.
+
+Lemma sort_inv n m : Sort n === Sort m -> n = m.
+Proof.
+  intros.
+  apply church_rosser in H.
+  inv H.
+  apply red_sort_inv in H0.
+  apply red_sort_inv in H1.
+  subst; inv H1; eauto.
+Qed.
+
+Lemma prod_inv A1 A2 B1 B2 :
+  Prod A1 B1 === Prod A2 B2 -> A1 === A2 /\ B1 === B2.
+Proof.
+  intros.
+  apply church_rosser in H.
+  inv H.
+  apply red_prod_inv in H0.
+  apply red_prod_inv in H1.
+  firstorder; subst.
+  inv H4; eauto using join_conv.
+  inv H4; eauto using join_conv.
+Qed.
+
+Inductive sub1 : term ->term -> Prop :=
+| sub1_refl A : sub1 A A
+| sub1_sort n m : n <= m -> sub1 (Sort n) (Sort m)
+| sub1_prod A B1 B2 : sub1 B1 B2 -> sub1 (Prod A B1) (Prod A B2).
+
+CoInductive sub (A B : term) : Prop :=
+| SubI A' B' : sub1 A' B' -> A === A' -> B' === B -> sub A B.
+Infix "<:" := sub (at level 50, no associativity) : coc_scope.
+
+Lemma sub1_sub A B : sub1 A B -> sub A B. move=> /SubI. exact. Qed.
+Lemma sub1_conv B A C : sub1 A B -> B === C -> A <: C. move=>/SubI. exact. Qed.
+Lemma conv_sub1 B A C : A === B -> sub1 B C -> A <: C. move=>c/SubI. exact. Qed.
+
+Lemma conv_sub A B : A === B -> A <: B.
+Proof. move/conv_sub1. apply. exact: sub1_refl. Qed.
+
+Lemma sub_refl A : A <: A.
+Proof. apply: sub1_sub. exact: sub1_refl. Qed.
+Hint Resolve sub_refl.
+
+Lemma sub_sort n m : n <= m -> Sort n <: Sort m.
+Proof. move=> leq. exact/sub1_sub/sub1_sort. Qed.
+
+Lemma sub1_trans A B C D :
+  sub1 A B -> B === C -> sub1 C D -> A <: D.
+Proof with eauto using sub1, sub1_sub, sub1_conv, conv_sub1.
+  move=> sb. elim: sb C D => {A B}
+    [A C D|n m leq C D conv sb|A B1 B2 sb1 ih C D conv sb2]...
+  - inv sb...
+    + apply: sub_sort. move: conv => /sort_inv eqn. subst.
+      exact: leq_trans leq _.
+    + exfalso; solve_conv.
+  - inv sb2...
+    + exfalso; solve_conv.
+    + move: conv => /prod_inv[conv1 conv2].
+      move: (ih _ _ conv2 H) => {ih} sub. inv sub.
+      eapply SubI. eapply sub1_prod... eapply conv_prod... exact: conv_prod.
+Qed.
+
+Lemma sub_trans B A C :
+  A <: B -> B <: C -> A <: C.
+Proof.
+  move=> [A' B' s1 c1 c2] [B'' C' s2 c3 c4]. move: (conv_trans _ c2 c3) => h.
+  case: (sub1_trans s1 h s2) => A0 B0 s3 c5 c6. apply: (SubI s3).
+  exact: conv_trans c5. exact: conv_trans c4.
+Qed.
+
+Lemma sub1_subst sigma A B : sub1 A B -> sub1 A.[sigma] B.[sigma].
+Proof. move=> s. elim: s sigma => /=; eauto using sub1. Qed.
+
+Lemma sub_subst sigma A B : A <: B -> A.[sigma] <: B.[sigma].
+Proof. move=> [A' B' /sub1_subst]; eauto using sub, conv_subst. Qed.
+
+Reserved Notation "[ Gamma |- ]".
+Reserved Notation "[ Gamma |- s :- A ]".
+
+Inductive has_type : context term -> term -> term -> Prop :=
+| ty_sort Gamma n  :
+  [ Gamma |- Sort n :- Sort n.+1 ]
+| ty_prod Gamma A B n :
+  [ Gamma |- A :- Sort n ] ->
+  [ A :s Gamma |- B :- Sort n ] ->
+  [ Gamma |- Prod A B :- Sort n ]
+| ty_var Gamma x A :
+  has Gamma x A ->
+  [ Gamma |- Var x :- A ]
+| ty_lam Gamma A B s n :
+  [ Gamma |- Prod A B :- Sort n ] ->
+  [ A :s Gamma |- s :- B ] ->
+  [ Gamma |- Lam s :- Prod A B ]
+| ty_app Gamma A B s t :
+  [ Gamma |- s :- Prod A B ] ->
+  [ Gamma |- t :- A ] ->
+  [ Gamma |- App s t :- B.[t/] ]
+| ty_conv Gamma A B s n :
+  A <: B ->
+  [ Gamma |- B :- Sort n ] ->
+  [ Gamma |- s :- A ] ->
+  [ Gamma |- s :- B ]
+where "[ Gamma |- s :- A ]" := (has_type Gamma s A).
+
+Inductive context_ok : context term -> Prop :=
+| nil_ok :
+  [ nil |- ]
+| s_ok Gamma A n :
+  [ Gamma |- A :- Sort n ] ->
+  [ Gamma |- ] ->
+  [ A :s Gamma |- ]
+| n_ok Gamma :
+  [ Gamma |- ] ->
+  [ :n Gamma |- ]
+where "[ Gamma |- ]" := (context_ok Gamma).
+
+Notation "[ Gamma |- s ]" := (exists n, [ Gamma |- s :- Sort n ]).
+
+Inductive agree_ren : (var -> var) ->
+  context term -> context term -> Prop :=
+| agree_ren_nil xi :
+  agree_ren xi nil nil
+| agree_ren_s Gamma Gamma' xi m :
+  agree_ren xi Gamma Gamma' ->
+  agree_ren (upren xi) (m :s Gamma) (m.[ren xi] :s Gamma')
+| agree_ren_n Gamma Gamma' xi :
+  agree_ren xi Gamma Gamma' ->
+  agree_ren (upren xi) (:n Gamma) (:n Gamma')
+| agree_ren_wk Gamma Gamma' xi m :
+  agree_ren xi Gamma Gamma' ->
+  agree_ren ((+1) ∘ xi) (Gamma) (m :: Gamma').
+
+Lemma agree_ren_refl Gamma :
+  agree_ren id Gamma Gamma.
+Proof.
+  induction Gamma.
+  - constructor.
+  - destruct a. 
+    assert (agree_ren id (t :s Gamma) (t :s Gamma)
+      = agree_ren (upren id) (t :s Gamma) (t.[ren id] :s Gamma))
+      by autosubst.
+    rewrite H.
+    constructor; eauto.
+    assert (agree_ren id (:n Gamma) (:n Gamma)
+      = agree_ren (upren id) (:n Gamma) (:n Gamma))
+      by autosubst.
+    rewrite H.
+    constructor; eauto.
+Qed.
+
+Lemma agree_ren_has Gamma Gamma' xi :
+  agree_ren xi Gamma Gamma' ->
+  forall x A,
+    has Gamma x A ->
+    has Gamma' (xi x) A.[ren xi].
+Proof.
+  intro H2.
+  dependent induction H2; simpl; intros; eauto.
+  - inv H.
+  - destruct x; asimpl.
+    inv H.
+    replace (m.[ren (+1)].[ren (upren xi)]) 
+      with (m.[ren xi].[ren (+1)]) by autosubst.
+    constructor.
+    inv H; subst.
+    replace (m0.[ren (+1)].[ren (upren xi)]) 
+      with (m0.[ren xi].[ren (+1)]) by autosubst.
+    constructor.
+    apply IHagree_ren; eauto.
+  - inv H; subst.
+    replace (m.[ren (+1)].[ren (upren xi)]) 
+      with (m.[ren xi].[ren (+1)]) by autosubst.
+    constructor.
+    apply IHagree_ren; eauto.
+  - replace (A.[ren ((+1) ∘ xi)])
+      with (A.[ren xi].[ren (+1)]) by autosubst.
+    destruct m; constructor; apply IHagree_ren; eauto.
+Qed.
+
+Lemma rename_ok Gamma m A :
+  [ Gamma |- m :- A ] ->
+  forall Gamma' xi,
+    agree_ren xi Gamma Gamma' ->
+    [ Gamma' |- m.[ren xi] :- A.[ren xi] ].
+Proof.
+  intros H.
+  induction H; simpl; intros.
+  - apply ty_sort; assumption.
+  - asimpl.
+    apply ty_prod; eauto.
+    replace (Sort n) with ((Sort n).[ren (upren xi)]) by autosubst.
+    apply IHhas_type2.
+    constructor; eauto.
+  - replace (ids (xi x)) with (Var (xi x)) by autosubst.
+    apply ty_var.
+    eapply agree_ren_has; eauto.
+  - eapply ty_lam.
+    apply IHhas_type1; eauto.
+    asimpl.
+    apply IHhas_type2; eauto.
+    constructor; eauto.
+  - asimpl.
+    specialize (IHhas_type1 _ _ H1).
+    specialize (IHhas_type2 _ _ H1).
+    asimpl in IHhas_type1.
+    replace (B.[t.[ren xi] .: ren xi]) 
+      with (B.[ren (upren xi)].[t.[ren xi]/]) by autosubst.
+    eapply ty_app; eauto.
+  - eapply ty_conv.
+    apply sub_subst; eauto.
+    apply IHhas_type1; eauto.
+    apply IHhas_type2; eauto.
+Qed.
+
+Theorem weakening Gamma s A B :
+  [ Gamma |- s :- A ] -> 
+  [ B :: Gamma |- s.[ren (+1)] :- A.[ren (+1)] ].
+Proof.
+  intros.
+  eapply rename_ok in H.
+  apply H.
+  apply agree_ren_wk.
+  apply agree_ren_refl.
+Qed.
+
+Close Scope coc_scope.
+
+End ECC.
